theories/case_studies/multiuser_kvs/kvs_adequacy.v
@@ -30,8 +30,8 @@ Class memory_layout `{MP: MachineParameters} := {
     ot_kvs_size : (ot_kvs < ot_kvs ^+ 1)%ot;
     ot_kvs_disjoint : ot_kvs ≠ (ot_switcher switcher_cmpt) ;
 
-    kvs_user_key_K : Z;
-    kvs_user_key_B : Z;
+    kvs_user_key_K : user_key_t;
+    kvs_user_key_B : user_key_t;
     kvs_user_key_disjoints : kvs_user_key_K ≠ kvs_user_key_B;
 
     (* adv compartments B *)
@@ -226,11 +226,8 @@ Section Adequacy.
   Local Notation kvs_user_key_K_a := (0 ^+ kvs_user_key_K)%a.
   Local Notation kvs_user_key_B_a := (0 ^+ kvs_user_key_B)%a.
 
-  Context {kvs_preg: gen_heapGpreS nat kvs_entry Σ}.
-  Context {kvs_alloc_preg: gen_heapGpreS Z (gset Z) Σ}.
-  (* Context {KVS_users: kvs_users}. *)
-  (* Context { Hkvs_users_seals : kvs_users_seals = {[ B := kvs_user_key_B ]} }. *)
-  (* Context { Hkvs_users_seals_reserved : kvs_users_seals_reserved = [kvs_user_key_K] }. *)
+  Context {kvs_alloc_preg: gen_heapGpreS user_key_t kvs_user_map Σ}.
+  Context {kvs_logical_user_preg : ghost_mapG Σ user_key_t (option Word) }.
 
   Definition flagN : namespace := nroot .@ "kvs" .@ "fail_flag".
   Definition switcherN : namespace := nroot .@ "kvs" .@ "switcher_flag".
@@ -323,7 +320,11 @@ Section Adequacy.
 
     assert kvs_namespaces as kvs_namespacesg.
     {
-      refine (Build_kvs_namespaces (kvsN .@ "Nkvs") (kvsN .@ "Nkvs_otype") (kvsN .@ "Nkvs_exp_tbl") _).
+      refine (Build_kvs_namespaces
+                (kvsN .@ "Nkvs")
+                (kvsN .@ "Nkvs_otype")
+                (kvsN .@ "Nkvs_exp_tbl")
+                _).
       split;try solve_ndisj.
     }
     assert kvsLayoutWf as kvsLayoutWfg.
@@ -345,18 +346,29 @@ Section Adequacy.
     }
 
     set (all_users_keys := [kvs_user_key_K;kvs_user_key_B]).
-    set (kvs_alloc_init := (list_to_map ( (fun k => (k,∅)) <$> all_users_keys) : kvs_alloc)).
-    iMod (gen_heap_init (kvs_alloc_init : kvs_alloc)) as (kvs_alloc_heapg) "(Hkvs_alloc_auth & Hkvs_alloc_frag & _)".
-    assert ( kvs_alloc_init = {[ kvs_user_key_K := ∅ ; kvs_user_key_B := ∅ ]} ) as ->.
-    { subst kvs_alloc_init all_users_keys; done. }
+    set (lkvs_init := (list_to_map ( (fun k => (k,∅)) <$> all_users_keys) : kvs_logical_map)).
+    iMod (gen_heap_init (lkvs_init : kvs_logical_map))
+      as (kvs_logical_heapg) "(Hlkvs_auth & Hlkvs_frag & _)".
+    assert ( lkvs_init = {[ kvs_user_key_K := ∅ ; kvs_user_key_B := ∅ ]} ) as ->.
+    { subst lkvs_init all_users_keys; done. }
     assert ( kvs_user_key_K ≠ kvs_user_key_B ) as Huser_keys_disjoint.
     { pose proof kvs_user_key_disjoints; solve_addr. }
     rewrite (big_sepM_insert _ _ kvs_user_key_K); last by simplify_map_eq.
     rewrite (big_sepM_insert _ _ kvs_user_key_B); last by simplify_map_eq.
-    iDestruct "Hkvs_alloc_frag" as "(Halloc_K & Halloc_B & _)".
-    iMod (gen_heap_init (kvs_map_init : kvs_map)) as (kvs_heapg) "(Hkvs_auth & Hkvs_frags & _)".
+    iDestruct "Hlkvs_frag" as "(Hm_K & Hm_B & _)".
+    pose kvslogicalg := LogicalKvsG Σ kvs_logical_heapg.
 
-    pose kvsg := KvsG Σ kvs_heapg kvs_alloc_heapg.
+    iMod ( kvs_logical_user_init_pre {[ kvs_user_key_K ; kvs_user_key_B ]} kvs_logical_user_map_init) as (γf) "Hlukvs".
+    pose kvsuserg := UserKvsG Σ kvs_logical_user_preg γf.
+    pose kvsg := KvsG Σ kvslogicalg kvsuserg.
+    iDestruct (big_sepS_delete _ _ kvs_user_key_K with "Hlukvs")
+      as "[ [HK_lukvs_auth HK_lukvs_frag] Hlukvs]"; first by set_solver+.
+    iDestruct (big_sepS_delete _ _ kvs_user_key_B with "Hlukvs")
+      as "[ [HB_lukvs_auth HB_lukvs_frag] _]"; first by set_solver+Huser_keys_disjoint.
+    iDestruct (kvs_logical_user_map_init_None kvs_user_key_K with "[HK_lukvs_frag]") as "HK_lukvs_frag".
+    { cbn; iFrame. }
+    iDestruct (kvs_logical_user_map_init_None kvs_user_key_B with "[HB_lukvs_frag]") as "HB_lukvs_frag".
+    { cbn; iFrame. }
 
     pose proof (
         @kvs_main_spec Σ ceriseg seal_storeg _ _ _ _ _ _ _
@@ -452,13 +464,6 @@ Section Adequacy.
     set (kvs_erase' := (SCap RO Local _ _ (cmpt_exp_tbl_pcc kvs_cmpt ^+ kvs_erase_exp_tbl_off)%a)).
     clear Hneq_Bf_kvs_addOrUpdate Hneq_Bf_kvs_read Hneq_Bf_kvs_erase
       Hneq_kvs_addOrUpdate_kvs_read Hneq_kvs_addOrUpdate_kvs_erase Hneq_kvs_read_kvs_erase.
-
-
-    (* Notations *)
-    iAssert (◯(ALLOC)[ kvs_user_key_K ] ∅)%I with "Halloc_K" as "Halloc_K".
-    iAssert (◯(ALLOC)[ kvs_user_key_B ] ∅)%I with "Halloc_B" as "Halloc_B".
-    iAssert (●(ALLOC) {[kvs_user_key_K := ∅; kvs_user_key_B := ∅]})%I with "Hkvs_alloc_auth" as "Hkvs_alloc_auth".
-    iDestruct (kvs_initial_map_init_None with "[Hkvs_frags]") as "Hkvs_frags"; first iFrame.
 
     (* Get initial sregister mtdc *)
     iDestruct (big_sepM_lookup with "Hsreg") as "Hmtdc"; eauto.
@@ -597,25 +602,29 @@ Section Adequacy.
     iMod (seal_store_update_alloc _ ( kvs_otype_propC ) with "Hseal_store_kvs") as "#Hsealed_pred_ot_kvs".
 
     iMod (na_inv_alloc cerise_nais _ Nkvs kvs_inv
-           with "[Hkvs_auth Hkvs_frags Hkvs_alloc_auth Hkvs_imports Hkvs_data Hkvs_code]") as "#Hkvs".
+           with "[Hlkvs_auth Hkvs_imports Hkvs_data Hkvs_code]") as "#Hkvs".
     { iNext.
       rewrite /kvs_inv.
       rewrite kvs_data /kvs_data.
       pose proof (cmpt_data_size kvs_cmpt) as H.
       rewrite kvs_data /kvs_data in H.
       iFrame "∗#".
-      iSplit.
-      { iPureIntro; apply wf_kvs_map_kvs_map_init. }
+      rewrite /is_logical_kvs.
+      iExists kvs_physical_map_init.
       iSplit.
       { iPureIntro; apply kvs_alloc_synced_map_init.
         intros ku sk Hsk.
         clear -Hsk.
         by destruct (decide (ku = kvs_user_key_K)); simplify_map_eq.
       }
+      iSplit.
+      { iPureIntro; apply wf_kvs_physical_map_kvs_physical_map_init. }
       iEval (cbn).
-      iApply (kvs_initial_map_init with "[$] [Hkvs_frags]"); last iFrame.
-      rewrite /SIZE_MAP; solve_addr+H.
+      iApply (kvs_initial_map_init with "Hkvs_data"); rewrite /SIZE_MAP; solve_addr+H.
     }
+
+    iAssert (logical_user_kvs_inv kvs_user_key_K) with "[$Hm_K $HK_lukvs_auth]" as "Hkvs_logical_user_K".
+    { iPureIntro; apply kvs_synced_logical_user_kvs_init. }
 
     (* Initialises the world for B *)
 
@@ -634,8 +643,6 @@ Section Adequacy.
       pose proof (cmpt_exp_tbl_pcc_size kvs_cmpt) as H0.
       pose proof (cmpt_exp_tbl_cgp_size kvs_cmpt) as H1.
       pose proof (cmpt_exp_tbl_entries_size kvs_cmpt) as H2.
-      replace (cmpt_exp_tbl_entries_start kvs_cmpt)
-        with ((cmpt_exp_tbl_pcc kvs_cmpt) ^+ 2)%a by solve_addr+H0 H1.
       replace (cmpt_exp_tbl_cgp kvs_cmpt)
         with (cmpt_exp_tbl_pcc kvs_cmpt ^+ 1)%a by solve_addr+H0.
       iApply kvs_addOrUpdate_entry_point_spec; try iFrame "#"; eauto.
@@ -646,8 +653,6 @@ Section Adequacy.
       pose proof (cmpt_exp_tbl_pcc_size kvs_cmpt) as H0.
       pose proof (cmpt_exp_tbl_cgp_size kvs_cmpt) as H1.
       pose proof (cmpt_exp_tbl_entries_size kvs_cmpt) as H2.
-      replace (cmpt_exp_tbl_entries_start kvs_cmpt)
-        with ((cmpt_exp_tbl_pcc kvs_cmpt) ^+ 2)%a by solve_addr+H0 H1.
       replace (cmpt_exp_tbl_cgp kvs_cmpt)
         with (cmpt_exp_tbl_pcc kvs_cmpt ^+ 1)%a by solve_addr+H0.
       iApply kvs_read_entry_point_spec; try iFrame "#"; eauto.
@@ -658,8 +663,6 @@ Section Adequacy.
       pose proof (cmpt_exp_tbl_pcc_size kvs_cmpt) as H0.
       pose proof (cmpt_exp_tbl_cgp_size kvs_cmpt) as H1.
       pose proof (cmpt_exp_tbl_entries_size kvs_cmpt) as H2.
-      replace (cmpt_exp_tbl_entries_start kvs_cmpt)
-        with ((cmpt_exp_tbl_pcc kvs_cmpt) ^+ 2)%a by solve_addr+H0 H1.
       replace (cmpt_exp_tbl_cgp kvs_cmpt)
         with (cmpt_exp_tbl_pcc kvs_cmpt ^+ 1)%a by solve_addr+H0.
       iApply kvs_erase_entry_point_spec; try iFrame "#"; eauto.
@@ -695,15 +698,19 @@ Section Adequacy.
     set ( adversary_kvs_keys := ( {[ WSealable kvs_user_key_B_sb ; WSealable kvs_user_key_B_sb']} : gset Word)).
     set (W1' := <o[ ot_kvs := adversary_kvs_keys ]o> W1).
 
-    iAssert (kvs_otype_prop W1' B (WSealable kvs_user_key_B_sb)) with "[Halloc_B Ha_user_key_B]" as "ot_kvs_user_key_B".
+    iAssert (kvs_otype_prop W1' B (WSealable kvs_user_key_B_sb))
+      with "[$Hm_B $Ha_user_key_B $HB_lukvs_auth HB_lukvs_frag]" as "ot_kvs_user_key_B".
     {
-      iEval (rewrite /kvs_otype_prop /kvs_otype_inv /=).
-      iFrame "Halloc_B Ha_user_key_B".
-      repeat iSplit; auto; iPureIntro; try lia.
-      subst user_key_addr_B.
-      pose proof (cmpt_static_sealed_size B_cmpt) as H.
-      rewrite B_static_sealed in H.
-      solve_addr+H.
+      repeat iSplit.
+      - iPureIntro; auto.
+      - iPureIntro.
+        subst user_key_addr_B.
+        pose proof (cmpt_static_sealed_size B_cmpt) as H.
+        rewrite B_static_sealed in H.
+        solve_addr+H.
+      - iPureIntro; by apply kvs_synced_logical_user_kvs_init.
+      - iApply (big_sepS_impl with "HB_lukvs_frag").
+        iModIntro; iIntros (mk Hmk) "$".
     }
 
     assert (ot_kvs ∉ dom (seal_std W1)) as Hot_notin_W1.
@@ -921,6 +928,9 @@ Section Adequacy.
       ; first set_solver+.
       iApply interp_monotone_sd; eauto.
     }
+    
+    iDestruct (big_sepS_elem_of _ _ 1%Z with "HK_lukvs_frag") as "HK_lukvs_1".
+    { eapply is_uint16_in_kvs_all_map_keys; split; rewrite /UINT16_MIN /UINT16_MAX; lia. }
 
     iClear "HB_etbl_pcc HB_etbl_cgp HB_etbl_B_f HB_code HB_data Hinterp_pcc_B Hinterp_cgp_B".
 
@@ -936,11 +946,11 @@ Section Adequacy.
     iPoseProof (Spec _ _ _ _ _ _ _ _ _ _
                   _ _ _ _ _ _
                   [] [] [] assertN switcherN
-                 with "[ $Hassert $Hswitcher $Hkvs
+                 with "[ $Hassert $Hswitcher $Hkvs $Hkvs_logical_user_K
                         $Hkvs_etbl_pcc $Hkvs_etbl_cgp $Hkvs_etbl_entries_addOrUpdate $Hkvs_etbl_entries_read
                         $Hna $HPC $Hcgp $Hcsp $Hreg
                         $Hmain_imports $Hmain_code $Hmain_data $Hmain_static_sealed
-                        $Halloc_K
+                        $HK_lukvs_1
                         $Hworld_B $Hcstk_frag
                         $Hinterp_B_f $Hentry_Bf $Hinterp_stack_B
                         ]") as "Hspec"; eauto.
@@ -1036,7 +1046,8 @@ Proof.
               ; na_invΣ; sealStorePreΣ
               ; STS_preΣ Addr region_type OType Word ; relPreΣ
               ; savedPredΣ (WorldT * CmptName * Word)
-              ; gen_heapΣ nat kvs_entry ; gen_heapΣ Z (gset Z)
+              ; gen_heapΣ user_key_t kvs_user_map
+              ; ghost_mapΣ user_key_t (option Word)
       ]).
   eapply (@kvs_adequacy' Σ cnames B); eauto; try typeclasses eauto.
 Qed.
